CheckArith/Stmt.v
@@ -1,0 +1,805 @@
+From Coq Require Import Arith NArith ZArith Lia String Eqdep_dec.
+
+From Vyper Require Import Logic2.
+From Vyper Require Import Config L10.Base Calldag.
+From Vyper Require OpenArray.
+From Vyper Require Import UInt256.
+From Vyper.CheckArith Require Import CheckedArith Translate Builtins.
+From Vyper.L30 Require Import AST Stmt Callset VarCap.
+
+(** Two open arrays have the same [count] first elements. *)
+Definition MemoryPrefixAgree {C: VyperConfig} (mem1 mem2: memory) (count: N)
+:= let _ := memory_impl in
+   forall n: N,
+     (n < count)%N
+      ->
+     OpenArray.get mem1 n = OpenArray.get mem2 n.
+
+
+(** Replace [ view ... ... 1 ] with [get ... :: nil].
+    This is basically the same as [rewrite OpenArray.view1],
+    except it avoids the annoying "metavariable has several occurences" error.
+ *)
+Ltac view1
+:= let a := fresh "a" in
+   let v := fresh "v" in
+   let LenOk := fresh "LenOk" in
+   let Eqn := fresh "Eqn" in
+   let OkA := fresh "OkA" in
+   match goal with
+   |- context [ @OpenArray.view ?ValueType ?Zero ?MemType ?MemClass ?memory ?offset 1%N ] =>
+       remember (OpenArray.view memory offset 1%N) as v eqn:Eqn;
+       assert (LenOk := @OpenArray.view_len ValueType Zero MemType MemClass memory offset 1%N);
+       destruct v as [|a]; try discriminate;
+       destruct v; try discriminate;
+       clear LenOk;
+       (* Eqn is now [a :: nil = view ... ... 1] *)
+       assert (OkA := @OpenArray.view_ok ValueType Zero MemType MemClass memory offset 1 0 N.lt_0_1);
+       rewrite<- Eqn in OkA; clear Eqn;
+       rewrite N.add_0_r in OkA;
+       replace (List.nth_error (a :: nil) (N.to_nat 0)) with (Some a) in OkA by trivial;
+       inversion OkA; subst a; clear OkA
+   end.
+
+(** Replace [ view ... ... 2 ] with [get ... :: get ... :: nil].
+    This is basically the same as [rewrite OpenArray.view2],
+    except it avoids the annoying "metavariable has several occurences" error.
+ *)
+Ltac view2
+:= let a := fresh "a" in
+   let b := fresh "b" in
+   let v := fresh "v" in
+   let LenOk := fresh "LenOk" in
+   let Eqn := fresh "Eqn" in
+   let OkA := fresh "OkA" in
+   let OkB := fresh "OkB" in
+   match goal with
+   |- context [ @OpenArray.view ?ValueType ?Zero ?MemType ?MemClass ?memory ?offset 2%N ] =>
+       remember (OpenArray.view memory offset 2%N) as v eqn:Eqn;
+       assert (LenOk := @OpenArray.view_len ValueType Zero MemType MemClass memory offset 2%N);
+       destruct v as [|a]; try discriminate;
+       destruct v as [|b]; try discriminate;
+       destruct v; try discriminate;
+       clear LenOk;
+       (* Eqn is now [a :: b :: nil = view ... ... 2] *)
+       assert (OkA := @OpenArray.view_ok ValueType Zero MemType MemClass memory offset 2 0 N.lt_0_2);
+       assert (OkB := @OpenArray.view_ok ValueType Zero MemType MemClass memory offset 2 1 N.lt_1_2);
+       rewrite<- Eqn in OkA; rewrite<- Eqn in OkB; clear Eqn;
+       rewrite N.add_0_r in OkA; rewrite N.add_1_r in OkB;
+       replace (List.nth_error (a :: b :: nil) (N.to_nat 0)) with (Some a) in OkA by trivial;
+       replace (List.nth_error (a :: b :: nil) (N.to_nat 1)) with (Some b) in OkB by trivial;
+       inversion OkA; subst a; inversion OkB; subst b; clear OkA OkB
+   end.
+
+
+(* Convert a BuiltinsSupportBinop clause into BuiltinIsBinop;
+   pass the arity check and rewrite the builtin call.
+   Example: open_binop builtin_name_uint256_add binop_add.
+   Invoke after reducing the interpreted code to (builtins ...)
+*)
+Ltac do_binop selector newname
+:= let op_name := fresh newname in
+   let A := fresh "A" in
+   let arity := fresh "arity" in
+   let CondOk := fresh "CondOk" in
+   match goal with
+   | H: @BuiltinsSupportBinop ?C ?builtins (selector ?B) (?op ?C) |- _ =>
+      unfold BuiltinsSupportBinop in H;
+      destruct (builtins (selector B)) as [op_name|];
+      try contradiction;
+      assert (A := builtin_is_binop_arity _ _ H);
+      destruct op_name as (arity, op_name);
+      cbn in A;
+      subst arity;
+      match goal with
+      |- context [ 2 =? ?rhs = ?ok] =>
+          assert (CondOk: 2 =? rhs = true) by now rewrite OpenArray.view_len
+      end;
+      rewrite if_yes with (E := CondOk);
+      cbn in CondOk;
+      view2;
+      rewrite (builtin_is_binop_ok _ _ H);
+      clear CondOk
+   end.
+
+Ltac do_binop_nocbn selector newname
+:= let op_name := fresh newname in
+   let A := fresh "A" in
+   let arity := fresh "arity" in
+   let CondOk := fresh "CondOk" in
+   match goal with
+   | H: @BuiltinsSupportBinop ?C ?builtins (selector ?B) (?op ?C) |- _ =>
+      unfold BuiltinsSupportBinop in H;
+      destruct (builtins (selector B)) as [op_name|];
+      try contradiction;
+      assert (A := builtin_is_binop_arity _ _ H);
+      destruct op_name as (arity, op_name);
+      simpl in A;
+      subst arity;
+      match goal with
+      |- context [ 2 =? ?rhs = ?ok] =>
+          assert (CondOk: 2 =? rhs = true) by now rewrite OpenArray.view_len
+      end;
+      rewrite if_yes with (E := CondOk);
+      simpl in CondOk;
+      view2;
+      rewrite (builtin_is_binop_ok _ _ H);
+      clear CondOk
+   end.
+
+(* example: open_unop builtin_name_uint256_not binop_not. *)
+Ltac do_unop selector newname
+:= let op_name := fresh newname in
+   let A := fresh "A" in
+   let arity := fresh "arity" in
+   let CondOk := fresh "CondOk" in
+   match goal with
+   | H: @BuiltinsSupportUnop ?C ?builtins (selector ?B) (?op ?C) |- _ =>
+      unfold BuiltinsSupportUnop in H;
+      destruct (builtins (selector B)) as [op_name|];
+      try contradiction;
+      assert (A := builtin_is_unop_arity _ _ H);
+      destruct op_name as (arity, op_name);
+      cbn in A;
+      subst arity;
+      match goal with
+      |- context [ 1 =? ?rhs = ?ok] =>
+          assert (CondOk: 1 =? rhs = true) by now rewrite OpenArray.view_len
+      end;
+      rewrite if_yes with (E := CondOk);
+      cbn in CondOk;
+      view1;
+      rewrite (builtin_is_unop_ok _ _ H);
+      clear CondOk
+   end.
+
+Local Lemma lt_ne_helper (x y: N) (L: (x < y)%N):
+  (x =? y)%N = false.
+Proof. apply N.eqb_neq. lia. Qed.
+
+Local Lemma lt_ne_helper' (x y: N) (L: (x < y)%N):
+  (y =? x)%N = false.
+Proof. apply N.eqb_neq. lia. Qed.
+
+Local Lemma lt_ne1_helper (x y: N) (L: (x < y)%N):
+  (x =? N.succ y)%N = false.
+Proof. apply N.eqb_neq. lia. Qed.
+
+Local Lemma lt_ne1_helper' (x y: N) (L: (x < y)%N):
+  (N.succ y =? x)%N = false.
+Proof. apply N.eqb_neq. lia. Qed.
+
+Local Lemma lt_ne2_helper (x y: N) (L: (x < y)%N):
+  (x =? N.succ (N.succ y))%N = false.
+Proof. apply N.eqb_neq. lia. Qed.
+
+Local Lemma lt_ne2_helper' (x y: N) (L: (x < y)%N):
+  (N.succ (N.succ y) =? x)%N = false.
+Proof. apply N.eqb_neq. lia. Qed.
+
+Local Lemma noalias1 (x: N): (x =? N.succ x)%N = false.
+Proof. rewrite N.eqb_neq. lia. Qed.
+Local Lemma noalias2 (x: N): (x =? N.succ (N.succ x))%N = false.
+Proof. rewrite N.eqb_neq. lia. Qed.
+Local Lemma noalias1' (x: N): (N.succ x =? x)%N = false.
+Proof. rewrite N.eqb_neq. lia. Qed.
+Local Lemma noalias2' (x: N): (N.succ (N.succ x) =? x)%N = false.
+Proof. rewrite N.eqb_neq. lia. Qed.
+
+(* TODO: to Arith2 *)
+Lemma Z_ltb_succ_r (n m: Z):
+  ((n <? Z.succ m) = (n <=? m))%Z.
+Proof.
+apply (relation_quad Z.ltb_lt Z.leb_le).
+apply Z.lt_succ_r.
+Qed.
+
+Lemma translate_small_stmt_ok {C: VyperConfig}
+                              {bigger_call_depth_bound smaller_call_depth_bound: nat}
+                              (Ebound: bigger_call_depth_bound = S smaller_call_depth_bound)
+                              (builtins: string -> option builtin)
+                              (B: builtin_names_config)
+                              (scratch: N)
+                              (BuiltinsOk: BuiltinsSupportUInt256 B builtins)
+                              {cd: L30.Descend.calldag}
+                              (fc: fun_ctx cd bigger_call_depth_bound)
+                              {do_call': forall (fc': fun_ctx (translate_calldag B scratch cd)
+                                                              smaller_call_depth_bound)
+                                                (world: world_state)
+                                                (arg_values: list uint256),
+                                            world_state * expr_result uint256}
+                              {do_call: forall (fc': fun_ctx cd smaller_call_depth_bound)
+                                               (world: world_state)
+                                               (arg_values: list uint256),
+                                           world_state * expr_result uint256}
+                              (DoCallOk: forall fc' world arg_values,
+                                     do_call' (translate_fun_ctx B scratch fc') world arg_values
+                                      =
+                                     do_call fc' world arg_values)
+                              (ss: small_stmt)
+                              (CallOk': let _ := string_set_impl in 
+                                 FSet.is_subset (stmt_callset (translate_small_stmt B scratch ss))
+                                                (decl_callset
+                                                   (fun_decl
+                                                     (translate_fun_ctx B scratch fc)))
+                                 = true)
+                              (CallOk: let _ := string_set_impl in 
+                                 FSet.is_subset (small_stmt_callset ss)
+                                                (Callset.decl_callset (fun_decl fc))
+                                 = true)
+                              (world: world_state)
+                              (mem' mem: memory)
+                              (ScratchOk: (var_cap_small_stmt ss <= scratch)%N)
+                              (Agree: MemoryPrefixAgree mem' mem scratch):
+  let _ := string_map_impl in
+  let _ := memory_impl in
+  let '(w', m', result') := interpret_stmt Ebound (translate_fun_ctx B scratch fc)
+                                                  do_call' builtins
+                                                  world mem' (translate_small_stmt B scratch ss)
+                                                  CallOk' in
+  let '(w, m, result) := interpret_small_stmt Ebound fc do_call builtins world mem ss CallOk in
+    result' = result
+     /\
+    w' = w
+     /\
+    MemoryPrefixAgree m' m scratch.
+Proof.
+unfold BuiltinsSupportUInt256 in BuiltinsOk.
+destruct BuiltinsOk as (AddOk, (SubOk, (MulOk, (DivOk, (ModOk,
+                        (PowOk, (NotOk, (IsZeroOk, (AndOk, (OrOk, (XorOk,
+                         (LtOk, (EqOk, (ShlOk, ShrOk)))))))))))))).
+
+destruct ss; simpl; simpl in ScratchOk. (* cbn hangs up *)
+{ (* Pass *) easy. }
+{ (* Const *)
+  repeat (split; trivial).
+  intros n L.
+  repeat rewrite OpenArray.put_ok.
+  destruct (dst =? n)%N. { trivial. }
+  apply (Agree n L).
+}
+{ (* Copy *)
+  repeat (split; trivial).
+  intros n L.
+  repeat rewrite OpenArray.put_ok.
+  destruct (dst =? n)%N. { apply Agree. lia. }
+  apply (Agree n L).
+}
+{ (* StorageGet *)
+  assert (D := calldag_map_declmap (translate_decl B scratch)
+                                   (Translate.translate_calldag_helper B scratch cd)
+                                   cd name).
+  destruct (cd_declmap
+     (calldag_map (translate_decl B scratch) (Translate.translate_calldag_helper B scratch cd) cd)
+     name) as [d'|], (cd_declmap cd name) as [d|]; try discriminate.
+  2:easy. (* not found *)
+  destruct d; cbn in D; inversion D; subst d'.
+  2:easy. (* found but it's a function decl *)
+  repeat (split; trivial).
+  intros n L.
+  repeat rewrite OpenArray.put_ok.
+  destruct (dst =? n)%N. { trivial. }
+  apply (Agree n L).
+}
+{ (* StoragePut *)
+  assert (D := calldag_map_declmap (translate_decl B scratch)
+                                   (Translate.translate_calldag_helper B scratch cd)
+                                   cd name).
+  destruct (cd_declmap
+     (calldag_map (translate_decl B scratch) (Translate.translate_calldag_helper B scratch cd) cd)
+     name) as [d'|], (cd_declmap cd name) as [d|]; try discriminate.
+  2:easy. (* not found *)
+  destruct d; cbn in D; inversion D; subst d'.
+  2:easy. (* found but it's a function decl *)
+  repeat (split; trivial).
+  f_equal.
+  apply Agree. lia.
+}
+{ (* UnOp *)
+  destruct op.
+  { (* ~ *)
+    cbn.
+    do_unop builtin_name_uint256_not unop_not.
+    repeat (split; trivial).
+    intros n L.
+    repeat rewrite OpenArray.put_ok.
+    remember (dst =? n)%N as dst_n. symmetry in Heqdst_n.
+    destruct dst_n; [f_equal|]; apply Agree; lia.
+  }
+  { (* logical not (iszero) *)
+    cbn.
+    do_unop builtin_name_uint256_iszero unop_iszero.
+    repeat (split; trivial).
+    intros n L.
+    repeat rewrite OpenArray.put_ok.
+    remember (dst =? n)%N as dst_n. symmetry in Heqdst_n.
+    destruct dst_n; [f_equal|]; apply Agree; lia.
+  }
+  (* unary -, the stupidest operator *)
+  unfold Base.interpret_unop. rewrite<- uint256_checked_neg_ok.
+  unfold uint256_checked_neg.
+  cbn.
+  assert (E: let _ := memory_impl in OpenArray.get mem' src = OpenArray.get mem src).
+  { apply Agree. lia. }
+  rewrite E.
+  destruct (Z_of_uint256 (OpenArray.get mem src) =? 0)%Z.
+  {
+    repeat (split; trivial).
+    intros n L.
+    repeat rewrite OpenArray.put_ok.
+    remember (dst =? n)%N as dst_n. symmetry in Heqdst_n.
+    destruct dst_n; [f_equal|]; apply Agree; lia.
+  }
+  cbn.
+  repeat (split; trivial).
+  { now rewrite OpenArray.put_same. }
+  intros n L.
+  repeat rewrite OpenArray.put_ok.
+  remember (scratch =? n)%N as e. symmetry in Heqe.
+  destruct e. { rewrite N.eqb_eq in Heqe. lia. }
+  apply (Agree n L).
+}
+3:{ (* BinOp *)
+  unfold Base.interpret_binop.
+  assert (NoAliasDstScratch: (dst =? scratch)%N = false) by (rewrite N.eqb_neq; lia).
+  assert (NoAliasDstScratch1: (dst =? N.succ scratch)%N = false) by (rewrite N.eqb_neq; lia).
+  assert (NoAliasDstScratch2: (dst =? N.succ (N.succ scratch))%N = false) by (rewrite N.eqb_neq; lia).
+  assert (NoAliasScratchDst: (scratch =? dst)%N = false) by (rewrite N.eqb_neq; lia).
+  assert (NoAliasScratch1Dst: (N.succ scratch =? dst)%N = false) by (rewrite N.eqb_neq; lia).
+  assert (NoAliasScratch2Dst: (N.succ (N.succ scratch) =? dst)%N = false) by (rewrite N.eqb_neq; lia).
+  assert (NoAliasSrc1Scratch: (src1 =? scratch)%N = false) by (rewrite N.eqb_neq; lia).
+  assert (NoAliasSrc1Scratch1: (src1 =? N.succ scratch)%N = false) by (rewrite N.eqb_neq; lia).
+  assert (NoAliasSrc1Scratch2: (src1 =? N.succ (N.succ scratch))%N = false) by (rewrite N.eqb_neq; lia).
+  assert (NoAliasScratchSrc1: (scratch =? src1)%N = false) by (rewrite N.eqb_neq; lia).
+  assert (NoAliasScratch1Src1: (N.succ scratch =? src1)%N = false) by (rewrite N.eqb_neq; lia).
+  assert (NoAliasScratch2Src1: (N.succ (N.succ scratch) =? src1)%N = false) by (rewrite N.eqb_neq; lia).
+  assert (NoAliasSrc2Scratch: (src2 =? scratch)%N = false) by (rewrite N.eqb_neq; lia).
+  assert (NoAliasSrc2Scratch1: (src2 =? N.succ scratch)%N = false) by (rewrite N.eqb_neq; lia).
+  assert (NoAliasSrc2Scratch2: (src2 =? N.succ (N.succ scratch))%N = false) by (rewrite N.eqb_neq; lia).
+  assert (NoAliasScratchSrc2: (scratch =? src2)%N = false) by (rewrite N.eqb_neq; lia).
+  assert (NoAliasScratch1Src2: (N.succ scratch =? src2)%N = false) by (rewrite N.eqb_neq; lia).
+  assert (NoAliasScratch2Src2: (N.succ (N.succ scratch) =? src2)%N = false) by (rewrite N.eqb_neq; lia).
+
+  Local Ltac aliasing
+  := repeat (rewrite N.eqb_refl
+          || rewrite noalias1
+          || rewrite noalias2
+          || rewrite noalias1'
+          || rewrite noalias2'
+          || match goal with
+             | H: (_ =? _)%N = false |- _ => rewrite H
+             | H: forall x: N, (_ =? _)%N = false |- _ => rewrite H
+             | H: (?a < ?b)%N |- _ => rewrite (lt_ne_helper a b H)
+             | H: (?a < ?b)%N |- _ => rewrite (lt_ne1_helper a b H)
+             | H: (?a < ?b)%N |- _ => rewrite (lt_ne2_helper a b H)
+             | H: (?a < ?b)%N |- _ => rewrite (lt_ne_helper' a b H)
+             | H: (?a < ?b)%N |- _ => rewrite (lt_ne1_helper' a b H)
+             | H: (?a < ?b)%N |- _ => rewrite (lt_ne2_helper' a b H)
+             end).
+  assert (R1: let _ := memory_impl in OpenArray.get mem' src1 = OpenArray.get mem src1)
+    by (apply Agree; lia). cbn in R1.
+  assert (R2: let _ := memory_impl in OpenArray.get mem' src2 = OpenArray.get mem src2)
+    by (apply Agree; lia). cbn in R2.
+
+  destruct op.
+  { (* < *)
+    cbn.
+    do_binop builtin_name_uint256_lt binop_lt.
+    repeat (split; trivial).
+    intros n L.
+    repeat rewrite OpenArray.put_ok.
+    aliasing. destruct (dst =? n)%N; aliasing.
+    { f_equal; apply Agree; lia. }
+    apply (Agree n L).
+  }
+  { (* >= *)
+    cbn. rewrite uint256_le_ok.
+    do_binop builtin_name_uint256_lt binop_lt.
+    do_unop builtin_name_uint256_iszero unop_iszero.
+    repeat (split; trivial).
+    intros n L.
+    repeat rewrite OpenArray.put_ok.
+    destruct (dst =? n)%N; aliasing.
+    { f_equal. f_equal; apply Agree; lia. }
+    apply (Agree n L).
+  }
+  { (* > *)
+    cbn.
+    do_binop builtin_name_uint256_lt binop_lt.
+    repeat (split; trivial).
+    intros n L.
+    repeat rewrite OpenArray.put_ok.
+    destruct (dst =? n)%N; aliasing.
+    { rewrite uint256_gt_ok. f_equal; apply Agree; lia. }
+    apply (Agree n L).
+  }
+  { (* >= *)
+    cbn. rewrite uint256_ge_ok.
+    do_binop builtin_name_uint256_lt binop_lt.
+    do_unop builtin_name_uint256_iszero unop_iszero.
+    repeat (split; trivial).
+    intros n L.
+    repeat rewrite OpenArray.put_ok.
+    destruct (dst =? n)%N; aliasing.
+    { f_equal. f_equal; apply Agree; lia. }
+    apply (Agree n L).
+  }
+  { (* == *)
+    cbn.
+    do_binop builtin_name_uint256_eq binop_eq.
+    repeat (split; trivial).
+    intros n L.
+    repeat rewrite OpenArray.put_ok.
+    destruct (dst =? n)%N; aliasing.
+    { f_equal; apply Agree; lia. }
+    apply (Agree n L).
+  }
+  { (* != *)
+    cbn. rewrite uint256_ne_ok.
+    do_binop builtin_name_uint256_eq binop_eq.
+    do_unop builtin_name_uint256_iszero unop_iszero.
+    repeat (split; trivial).
+    intros n L.
+    repeat rewrite OpenArray.put_ok.
+    destruct (dst =? n)%N; aliasing.
+    { f_equal. f_equal; apply Agree; lia. }
+    apply (Agree n L).
+  }
+  { (* | *)
+    cbn.
+    do_binop builtin_name_uint256_or binop_or.
+    repeat (split; trivial).
+    intros n L.
+    repeat rewrite OpenArray.put_ok.
+    destruct (dst =? n)%N; aliasing.
+    { f_equal; apply Agree; lia. }
+    apply (Agree n L).
+  }
+  { (* & *)
+    cbn. do_binop builtin_name_uint256_and binop_and.
+    repeat (split; trivial).
+    intros n L.
+    repeat rewrite OpenArray.put_ok.
+    destruct (dst =? n)%N; aliasing.
+    { f_equal; apply Agree; lia. }
+    apply (Agree n L).
+  }
+  { (* ^ *)
+    cbn. do_binop builtin_name_uint256_xor binop_xor.
+    repeat (split; trivial).
+    intros n L.
+    repeat rewrite OpenArray.put_ok.
+    destruct (dst =? n)%N; aliasing.
+    { f_equal; apply Agree; lia. }
+    apply (Agree n L).
+  }
+  { (* << *)
+    cbn.
+    do_binop builtin_name_uint256_shl binop_shl.
+    replace (scratch + 2)%N with (N.succ (N.succ scratch)) by lia.
+    repeat rewrite OpenArray.put_ok. aliasing.
+    do_binop builtin_name_uint256_shr binop_shr.
+    repeat rewrite OpenArray.put_ok. aliasing.
+    do_binop builtin_name_uint256_eq binop_eq.
+    repeat rewrite OpenArray.put_ok. aliasing.
+    assert (E := let _ := memory_impl in
+                 uint256_checked_shl_ok (OpenArray.get mem' src1) (OpenArray.get mem' src2)).
+    unfold uint256_checked_shl in E.
+    unfold uint256_eq. cbn in E.
+    remember (Z_of_uint256
+         (uint256_shr (uint256_shl (OpenArray.get mem' src1) (OpenArray.get mem' src2))
+            (OpenArray.get mem' src2)) =? Z_of_uint256 (OpenArray.get mem' src1))%Z as q.
+    clear Heqq. unfold one256. unfold zero256.
+    destruct q; rewrite uint256_ok; cbn; rewrite<- R1; rewrite<- R2; rewrite<- E; cbn;
+      repeat (split; trivial); intros n L; repeat rewrite OpenArray.put_ok; aliasing.
+    1:destruct (dst =? n)%N; trivial.
+    all:apply (Agree n L).
+  }
+  { (* >> *)
+    cbn.
+    do_binop builtin_name_uint256_shr binop_shr.
+    assert (E := let _ := memory_impl in
+                 uint256_shr_ok (OpenArray.get mem' src1) (OpenArray.get mem' src2)).
+    cbn in E. rewrite R1 in E. rewrite R2 in E. rewrite<- E.
+    repeat (split; trivial); intros n L.
+    repeat rewrite OpenArray.put_ok. aliasing.
+    destruct (dst =? n)%N; [f_equal|]; apply Agree; lia.
+  }
+  { (* + *)
+    cbn.
+    do_binop builtin_name_uint256_add binop_add.
+    do_binop builtin_name_uint256_lt binop_lt.
+    replace (scratch + 2)%N with (N.succ (N.succ scratch)) by lia.
+    repeat rewrite OpenArray.put_ok. aliasing.
+    assert (E := let _ := memory_impl in
+                 uint256_checked_add_ok (OpenArray.get mem' src1) (OpenArray.get mem' src2)).
+    unfold uint256_checked_add in E.
+    cbn in E. rewrite R1 in E. rewrite R2 in E. rewrite<- E.
+    unfold uint256_lt.
+    rewrite Z.geb_leb.
+    rewrite Z.leb_antisym.
+    rewrite Bool.if_negb.
+    clear E.
+    rewrite R1. rewrite R2. unfold one256. unfold zero256.
+    destruct (Z_of_uint256 (uint256_add (OpenArray.get mem src1) (OpenArray.get mem src2)) <?
+               Z_of_uint256 (OpenArray.get mem src1))%Z; rewrite uint256_ok; cbn;
+      repeat (split; trivial); intros n L;
+      repeat rewrite OpenArray.put_ok; aliasing.
+    { apply (Agree n L). }
+    destruct (dst =? n)%N; [f_equal|]; apply Agree; lia.
+  }
+  { (* - *)
+    cbn.
+    do_binop builtin_name_uint256_lt binop_lt.
+    repeat rewrite OpenArray.put_ok. aliasing.
+    do_binop builtin_name_uint256_sub binop_sub.
+    replace (scratch + 2)%N with (N.succ (N.succ scratch)) by lia.
+    repeat rewrite OpenArray.put_ok. aliasing.
+    assert (E := let _ := memory_impl in
+                 uint256_checked_sub_ok (OpenArray.get mem' src1) (OpenArray.get mem' src2)).
+    unfold uint256_checked_sub in E.
+    cbn in E. rewrite R1 in E. rewrite R2 in E. rewrite<- E. clear E.
+    rewrite Z.geb_leb.
+    rewrite Z.leb_antisym.
+    rewrite Bool.if_negb.
+    unfold uint256_lt.
+    rewrite R1. rewrite R2. unfold one256. unfold zero256.
+    destruct (Z_of_uint256 (OpenArray.get mem src1) <? Z_of_uint256 (OpenArray.get mem src2))%Z;
+      rewrite uint256_ok; cbn;
+      repeat (split; trivial); intros n L;
+      repeat rewrite OpenArray.put_ok; aliasing;
+      destruct (dst =? n)%N.
+    3:f_equal.
+    all:apply (Agree n L).
+  }
+  { (* * *)
+    cbn.
+    do_binop builtin_name_uint256_mul binop_mul.
+    do_binop builtin_name_uint256_div binop_div.
+    replace (scratch + 2)%N with (N.succ (N.succ scratch)) by lia.
+    repeat rewrite OpenArray.put_ok. aliasing.
+    do_binop builtin_name_uint256_eq binop_eq.
+    repeat rewrite OpenArray.put_ok. aliasing.
+    assert (E := let _ := memory_impl in
+                 uint256_checked_mul_ok (OpenArray.get mem' src1) (OpenArray.get mem' src2)).
+    unfold uint256_checked_mul in E.
+    cbn in E. rewrite R1 in E. rewrite R2 in E. rewrite<- E. clear E.
+    unfold uint256_eq.
+    rewrite R1. rewrite R2. unfold one256. unfold zero256.
+    destruct (Z_of_uint256 (OpenArray.get mem src1) =? 0)%Z.
+    {
+      repeat (split; trivial). intros n L.
+      repeat rewrite OpenArray.put_ok. aliasing.
+      destruct (dst =? n)%N; trivial; apply (Agree n L).
+    }
+    unfold zero256. unfold one256.
+    destruct (Z_of_uint256
+         (uint256_div (uint256_mul (OpenArray.get mem src1) (OpenArray.get mem src2))
+            (OpenArray.get mem src1)) =? Z_of_uint256 (OpenArray.get mem src2))%Z;
+      rewrite uint256_ok; cbn; repeat (split; trivial); intros n L;
+      repeat rewrite OpenArray.put_ok; aliasing.
+      2:apply (Agree n L).
+      destruct (dst =? n)%N; trivial; apply (Agree n L).
+  }
+  { (* / *)
+    cbn.
+    rewrite R2.
+    assert (E := let _ := memory_impl in
+                 uint256_checked_div_ok (OpenArray.get mem' src1) (OpenArray.get mem' src2)).
+    unfold uint256_checked_div in E.
+    cbn in E. rewrite R1 in E. rewrite R2 in E. rewrite<- E. clear E.
+    destruct (Z_of_uint256 (OpenArray.get mem src2) =? 0)%Z.
+    {
+      cbn. rewrite OpenArray.put_ok. aliasing.
+      repeat (split; trivial); intros n L;
+        rewrite OpenArray.put_ok; aliasing.
+      apply (Agree n L).
+    }
+    do_binop builtin_name_uint256_div binop_div.
+    repeat rewrite OpenArray.put_ok. aliasing.
+    unfold uint256_eq.
+    repeat (split; trivial); intros n L;
+      repeat rewrite OpenArray.put_ok; aliasing.
+    destruct (dst =? n)%N. 2:apply (Agree n L).
+    now f_equal.
+  }
+  { (* % *)
+    cbn.
+    rewrite R2.
+    assert (E := let _ := memory_impl in
+                 uint256_checked_mod_ok (OpenArray.get mem' src1) (OpenArray.get mem' src2)).
+    unfold uint256_checked_mod in E.
+    cbn in E. rewrite R1 in E. rewrite R2 in E. rewrite<- E. clear E.
+    destruct (Z_of_uint256 (OpenArray.get mem src2) =? 0)%Z.
+    {
+      cbn. rewrite OpenArray.put_ok. aliasing.
+      repeat (split; trivial); intros n L;
+        rewrite OpenArray.put_ok; aliasing.
+      apply (Agree n L).
+    }
+    do_binop builtin_name_uint256_mod binop_mod.
+    repeat rewrite OpenArray.put_ok. aliasing.
+    unfold uint256_eq.
+    repeat (split; trivial); intros n L;
+      repeat rewrite OpenArray.put_ok; aliasing.
+    destruct (dst =? n)%N. 2:apply (Agree n L).
+    now f_equal.
+  }
+  (* ** between non-consts is not supported *)
+  contradiction.
+}
+{ (* PowConstBase *)
+  simpl in *. (* cbn hangs *)
+  assert (E := let _ := memory_impl in
+               uint256_checked_pow_const_base_ok base (OpenArray.get mem' exp)).
+  unfold uint256_checked_pow_const_base in E.
+  unfold Base.interpret_binop.
+   assert (R: let _ := memory_impl in OpenArray.get mem' exp = OpenArray.get mem exp)
+    by (apply Agree; lia). cbn in R.
+  rewrite R in E. rewrite<- E. clear E.
+  remember (Z_of_uint256 base =? 0)%Z as base0.
+  destruct base0.
+  { (* 0 ** _ *)
+    cbn.
+    do_unop builtin_name_uint256_iszero unop_iszero.
+    repeat (split; trivial); intros n L;
+      repeat rewrite OpenArray.put_ok; aliasing.
+    destruct (dst =? n)%N.
+    { unfold uint256_iszero. now rewrite R. }
+    apply (Agree n L).
+  }
+  remember (Z_of_uint256 base =? 1)%Z as base1.
+  destruct base1.
+  { (* 1 ** _ *)
+    cbn.
+    repeat (split; trivial); intros n L;
+      repeat rewrite OpenArray.put_ok; aliasing.
+    destruct (dst =? n)%N; trivial.
+    apply (Agree n L).
+  }
+  remember (Z_of_uint256 base =? 2)%Z as base2.
+  destruct base2.
+  { (* 2 ** _ *)
+    cbn.
+    do_binop builtin_name_uint256_lt binop_lt.
+    replace (scratch + 2)%N with (N.succ (N.succ scratch)) by lia.
+    repeat rewrite OpenArray.put_ok; aliasing.
+    do_binop builtin_name_uint256_shl binop_shl.
+    repeat rewrite OpenArray.put_ok; aliasing.
+    unfold uint256_lt. rewrite uint256_ok. cbn.
+    unfold one256. unfold zero256.
+    rewrite R.
+    destruct (Z_of_uint256 (OpenArray.get mem exp) <? 256)%Z;
+      rewrite uint256_ok; cbn;
+      repeat (split; trivial); intros n L;
+      repeat rewrite OpenArray.put_ok; aliasing.
+    {
+      destruct (dst =? n)%N; trivial.
+      apply (Agree n L).
+    }
+    apply (Agree n L).
+  }
+  (* _ ** _ *)
+  assert (BaseLower: (2 < Z_of_uint256 base)%Z).
+  {
+    symmetry in Heqbase0. apply Z.eqb_neq in Heqbase0.
+    symmetry in Heqbase1. apply Z.eqb_neq in Heqbase1.
+    symmetry in Heqbase2. apply Z.eqb_neq in Heqbase2.
+    assert (K := uint256_range base).
+    lia.
+  }
+  assert (MP := uint256_max_power_ok _ BaseLower). simpl in MP.
+  destruct MP as (MP, _).
+  assert (PowerUpper: (uint256_max_power (Z_of_uint256 base) < 256)%Z).
+  {
+    assert (D := Z.lt_ge_cases (uint256_max_power (Z_of_uint256 base)) 256%Z).
+    case D; clear D; intro D. { exact D. }
+    exfalso.
+    enough (Z.pow_pos 2 256 <= Z_of_uint256 base ^ uint256_max_power (Z_of_uint256 base))%Z by lia.
+    apply (Z.le_trans _ (Z_of_uint256 base ^ 256)).
+    {
+      rewrite Z.pow_pos_fold.
+      apply Z.pow_le_mono_l.
+      lia.
+    }
+    apply Z.pow_le_mono_r; lia.
+  }
+  simpl in *.
+  do_binop_nocbn builtin_name_uint256_lt binop_lt.
+  replace (scratch + 2)%N with (N.succ (N.succ scratch)) by lia.
+  repeat rewrite OpenArray.put_ok; aliasing.
+  unfold uint256_lt.
+  rewrite Z.leb_antisym.
+  rewrite Bool.if_negb.
+  do_binop_nocbn builtin_name_uint256_pow binop_pow.
+  repeat rewrite OpenArray.put_ok; aliasing.
+  replace (scratch =? exp)%N with false by (symmetry; rewrite N.eqb_neq; lia).
+  rewrite R.
+  rewrite uint256_ok.
+  assert (PowerLower: (0 <= uint256_max_power (Z_of_uint256 base))%Z) by apply binary_search_lower.
+  rewrite Z.mod_small by lia.
+  unfold one256. unfold zero256.
+  destruct (uint256_max_power (Z_of_uint256 base) <? Z_of_uint256 (OpenArray.get mem exp))%Z;
+    rewrite uint256_ok; simpl;
+    repeat (split; trivial); intros n L;
+    repeat rewrite OpenArray.put_ok; aliasing.
+  { apply (Agree n L). }
+  destruct (dst =? n)%N; trivial.
+  apply (Agree n L).
+}
+{ (* PowConstExp *)
+  simpl in *.
+  assert (E := let _ := memory_impl in
+               uint256_checked_pow_const_exponent_ok (OpenArray.get mem' base) exp).
+  unfold uint256_checked_pow_const_exponent in E.
+  unfold Base.interpret_binop.
+   assert (R: let _ := memory_impl in OpenArray.get mem' base = OpenArray.get mem base)
+    by (apply Agree; lia). cbn in R.
+  rewrite R in E. rewrite<- E. clear E.
+  remember (Z_of_uint256 exp =? 0)%Z as exp0.
+  destruct exp0.
+  {
+    simpl.
+    repeat (split; trivial); intros n L;
+    repeat rewrite OpenArray.put_ok.
+    destruct (dst =? n)%N; trivial.
+    apply (Agree n L).
+  }
+  remember (Z_of_uint256 exp =? 1)%Z as exp1.
+  destruct exp1.
+  {
+    simpl.
+    do_binop_nocbn builtin_name_uint256_pow binop_pow.
+    repeat (split; trivial); intros n L;
+    repeat rewrite OpenArray.put_ok. aliasing.
+    destruct (dst =? n)%N; trivial.
+    {
+      rewrite R.
+      symmetry in Heqexp1.
+      apply Z.eqb_eq in Heqexp1.
+      unfold uint256_pow.
+      unfold one256.
+      rewrite Heqexp1.
+      now rewrite uint256_ok.
+    }
+    apply (Agree n L).
+  }
+  simpl.
+  do_binop_nocbn builtin_name_uint256_lt binop_lt.
+  repeat rewrite OpenArray.put_ok. aliasing.
+  unfold uint256_lt.
+  rewrite R.
+  rewrite uint256_ok.
+  assert (ExpLower: (2 <= Z_of_uint256 exp)%Z).
+  {
+    assert (K := uint256_range exp). 
+    symmetry in Heqexp0. apply Z.eqb_neq in Heqexp0.
+    symmetry in Heqexp1. apply Z.eqb_neq in Heqexp1.
+    lia.
+  }
+  assert (BaseLower: (0 <= uint256_max_base (Z_of_uint256 exp))%Z) by apply binary_search_lower.
+  assert (BaseUpper: (uint256_max_base (Z_of_uint256 exp) <= 2 ^ 128)%Z).
+  {
+    assert (MB := uint256_max_base_ok _ ExpLower). simpl in MB.
+    destruct MB as (MB, _).
+    rewrite Z.pow_pos_fold in MB.
+    assert (D := Z.le_gt_cases (uint256_max_base (Z_of_uint256 exp)) (2 ^ 128) %Z).
+    case D; clear D; intro D. { exact D. }
+    exfalso.
+    enough (2 ^ 256 <= uint256_max_base (Z_of_uint256 exp) ^ Z_of_uint256 exp)%Z by lia.
+    replace (2 ^ 256)%Z with ((2 ^ 128) ^ 2)%Z by trivial.
+    apply (Z.le_trans _ ((2 ^ 128) ^ Z_of_uint256 exp)).
+    { apply Z.pow_le_mono_r; lia. }
+    apply Z.lt_le_incl.
+    apply Z.pow_lt_mono_l; lia.
+  }
+  rewrite Z.mod_small by lia.
+  do_binop_nocbn builtin_name_uint256_pow binop_pow.
+  repeat rewrite OpenArray.put_ok; aliasing.
+  rewrite Z_ltb_succ_r.
+  unfold zero256. unfold one256.
+  destruct (Z_of_uint256 (OpenArray.get mem base) <=? uint256_max_base (Z_of_uint256 exp))%Z;
+    repeat rewrite OpenArray.put_ok; rewrite uint256_ok; simpl; aliasing;
+    repeat (split; trivial); intros n L; repeat rewrite OpenArray.put_ok; aliasing;
+    destruct (dst =? n)%N; trivial; apply (Agree n L).
+}
